---
layout: post
title: "First-order Linear with Constant Coefficients: Behavior of Solutions, Use of Complex Methods."
date: 2019-6-4
---



## Steady-state Solution

This session we introduced a special form of first order linear ODE (sry the name is long) written in standard form{%include sidenote.html note="the standard form is $$y'+p(t)y=q(t)$$"%}:

$$
y'+ky=q(t)
$$

where $$p(t)$$ is a constant $$k$$ and does not change with input. The integrating factor $$u=e^{\int kdt}=e^{kt}$$, then  

$$
\begin{align}
(ye^{kt})'&=e^{kt}q(t)\\
ye^{kt}&=\int e^{kt}q(t)\ dt+C\\
y&=\underbrace{e^{-kt}\int e^{kt}q(t)\ dt}_{steady-state\ solution}+\underbrace{Ce^{-kt}}_{\rightarrow0\ as\ t\rightarrow\infty\\transient}
\end{align}
$$

The term $$Ce^{-kt}$$ goes to zero as $$t$$ goes to infinity, the rest is called steady-state solution or long-term solution.  A steady-state solution means in the long-run, no matter what the initial value $$C=y_0$$ will be, the solution $$y$$ will converge to the steady-state solution. 

### Superposition of input

In brief, superposition of input is saying when we have input $$q_1(t)$$, a response{% include sidenote.html note='another name for solution'%} $$y_1(t)$$ and another response $$q_2(t)$$ and another output $$y_2(t)$$. The input $$q_1+q_2$$ has the output $$y_1+y_2$$



## Sinusoidal Input 

Let's have a special form of constant coefficient ODE:

$$
y'+ky=kq_e(t)
$$

A subscript $$e$$ is just a reminder that we have a constant $$k$$ on it. Since we have already seen a linear input, the temperature and concentration model in [lecture3](./first_order_linear_odes), this time let our input to be a cosine function:

$$
y'+ky=k*\cos(\omega t)\tag{1}
$$

where $$\omega$$ stands for the "angular frequency" or "# complete oscillations in 2$$\pi$$". To make the integration explicit, note that it's not necessary to do this, we are going to "complexify"Â the problem by going into the complex domain. Remember

$$
\cos\theta+i\sin\theta=e^{i\theta}
$$

We will rewrite the problem (1) into 

$$
\tilde y'+k\tilde y=k*e^{i\omega t}\tag{2}
$$

The reason we change $$y$$ into $$\tilde y$$ is because $$\tilde y$$ contains the real and imaginary solutions, turning into the "whole" solution, and we *only* need the *real* part{%include sidenote.html note='proof to be added'%}. An intuitive way to see this is by *Superposition of input* we feed in another imaginary input to (1). So 

$$
\begin{align}
\tilde y'+k\tilde y&=k*e^{i\omega t}\tag{2}\\
(\tilde ye^{kt})'&=k*e^{(k+i\omega )t}\\
\tilde ye^{kt}&=\frac{k}{k+i\omega}e^{(k+i\omega )t}\\
\tilde y&=\frac{1}{1+\frac{i\omega}{k}}e^{(i\omega )t}\\
\end{align}
$$

Now there're two ways to separate this whole solution into a combo of real and complex. Last time when we multiply a complex conjugate of the denominator is by "going into" the *Cartesian*. Today we will go into *polar*. Before that we need to some properties of a complex number

### Complex Properties

Let $$\alpha=a+ib$$. 

1. First and foremost, define $$\alpha^{-1}$$ s.t. $$\alpha*\alpha^{-1}=1$$. 

   Proof: What's $$\alpha^{-1}$$?  Let $$\alpha^{-1}=c+id$$, then 

   $$
   \begin{array}{}
   \alpha\alpha^{-1}&=(a+ib)(c+id)\\
   &=ac-bd+i(ad+bc)\\
   \end{array}\tag{3}
   $$

   The real part is $$ac-bd$$ and the imaginary part is $$ad+bc$$, we know that this two shall sum to 1, so 

   $$
   \begin{array}{}
   ac-bd=1(1)\\
   ad+cd=0(2)
   \end{array}\\
   \begin{array}{}
   &(1)*-b:-abc+b^2d=-b\\
   +&(2)*a:a^2+abc=0\\
   \Rightarrow&
   a^2+b^2d=-b\\
   \Rightarrow&
   d=\frac{-b}{a^2+b^2}
   \end{array}\\
   $$

   Similarly,
   
   $$
   \begin{array}{}
   &(1)*a:a^2c-abd=a\\
   +&(2)*b:abd+b^2c=0\\
   \Rightarrow&
   c=\frac{a}{a^2+b^2}
   \end{array}\\
   $$

   So at last,

   $$
   \begin{align}
   \alpha^{-1}&=\frac{a}{a^2+b^2}-\frac{b}{a^2+b^2}i\\
   &=\frac{a-bi}{(a-bi)(a-bi)}\\
   &=\frac{1}{a-bi}\\
   &=\frac{1}{\alpha}
   \end{align}
   $$

2. $$\arg(\alpha\beta)=\arg(\alpha)+\arg(\beta)$$, for arbitrary complex number $$\alpha=a+bi,\beta=c+di$$ 

   Proof: Similar to $$\tan$$, $$\arctan$$ has the a similar property s.t. 

   $$
   \tan^{-1}(\alpha)+\tan^{-1}(\beta)=\frac{\alpha+\beta}{1-\alpha\beta}
   $$

   From (3) we know product of any two complex number can be expressed that way, then the argument(angle) of $$\alpha*\beta$$ is
   
   $$
   \arg(\alpha\beta)=\tan^{-1}(\frac{ad+bc}{ac-bd})
   $$

   This is equal to 
   
   $$
   \arg(\alpha)+\arg(\beta)=\tan^{-1}(\frac{b}{a})+\tan^{-1}(\frac{d}{c})
   $$

3. $$\arg(1/\alpha)=-\arg(\alpha)$$

   Proof: Let $$\alpha=a+bi$$, then $$\arg(\alpha)=\tan^{-1}(\frac{b}{a})$$. From the proof of 1 we see 
   
   $$
   \alpha^{-1}=\frac{a}{a^2+b^2}-\frac{b}{a^2+b^2}i\\
   $$

   So 

   $$
   \arg(1/\alpha)=\tan^{-1}(-\frac{b}{a})
   $$

   And $$\arctan$$ is an odd function. 

4. $$\arg(1/\alpha)+\arg(\alpha)=0$$. 

### Polar Form

Let's back to our whole solution 

$$
\tilde y=\frac{1}{1+\frac{i\omega}{k}}e^{(i\omega )t}
$$

Let's take a look on the coefficient individually. Let $$\phi$$ be the angle of the denominator, that is, $$\arg(1+\frac{\omega}{k}i)=\phi$$. Then $$\arg(\frac{1}{1+\frac{\omega}{k}I})=-\phi$$. And the modulus $$r$$ is $$\frac{1}{\sqrt{1+(\omega/k)^2}}$$ . So we can express the coefficient as 

$$
\frac{1}{\sqrt{1+(\omega/k)^2}}e^{-i\phi}
$$

Then 

$$
\begin{align}
\tilde y&=\frac{1}{\sqrt{1+(\omega/k)^2}}e^{-i\phi}*e^{i\omega t}\\
&=r*e^{i(\omega t-\phi)}\\
&\Rightarrow\\
y&=r*\cos(\omega t-\phi)\\
\end{align}
$$

$$\phi=\tan^{-1}(\omega/k)$$ is called the phase lag, the shift of the trigonometry function.  And $$r$$ is the amplitude. $$k$$ is the conductivity. When $$k$$ goes up, $$\phi$$ goes down. Then the phase lag is smaller, it means we can get the response sooner(??? Not sure).  

The Cartesian solution will be in the next note.